\documentclass{article}
\usepackage{ifthen}
\usepackage{epsfig}
\usepackage[utf8]{inputenc}
% Packages requested by user
\usepackage{amsmath}

\usepackage{newunicodechar}
  \newunicodechar{⁻}{${}^{-}$}% Superscript minus
  \newunicodechar{²}{${}^{2}$}% Superscript two
  \newunicodechar{³}{${}^{3}$}% Superscript three

\pagestyle{empty}
\begin{document}
$M==N$
\pagebreak

$M>N$
\pagebreak

$k^{th}$
\pagebreak

$m^{th}$
\pagebreak

$(x-x_t)^2*(y-y_t)*(z-z_t)^3/factorial(2+1+3)$
\pagebreak

$(x_t,y_t,z_t)$
\pagebreak

$ N(i,j+1) $
\pagebreak

$ j^{th} $
\pagebreak

$ i $
\pagebreak

$ N(i,0) $
\pagebreak

$NB_d=$
\pagebreak

$d$
\pagebreak

$NB_{(d-1)/v}=$
\pagebreak

$(d-1)$
\pagebreak

$NB_d$
\pagebreak

\[\begin{bmatrix}b_i\\ -\int \frac{\partial}{\partial x}(b_i)\; dy\end{bmatrix},\]
\pagebreak

$i$
\pagebreak

$NB_{(d-1)/y}$
\pagebreak

\[\begin{bmatrix}0\\b_j\end{bmatrix},\]
\pagebreak

$j$
\pagebreak

$x$
\pagebreak

\[\begin{bmatrix}b_i\\ 0 \\-\int \frac{\partial}{\partial x}(b_i)\; dz\end{bmatrix},\]
\pagebreak

\[\begin{bmatrix}0\\ b_i \\-\int \frac{\partial}{\partial y}(b_i)\; dz\end{bmatrix},\]
\pagebreak

$NB_{(d-1)/z}$
\pagebreak

\[\begin{bmatrix}0\\0\\b_j\end{bmatrix},\]
\pagebreak

$y$
\pagebreak

\[\sum_{n=0}^{n=P} \frac{(x/h)^n}{n!}\]
\pagebreak

\[\sum_{n=0}^{n=P} \sum_{k=0}^{k=n} \frac{(x/h)^{n-k}*(y/h)^k}{(n-k)!k!}\]
\pagebreak

\[\sum_{p=0}^{p=P} \sum_{k_1+k_2+k_3=n} \frac{(x/h)^{k_1}*(y/h)^{k_2}*(z/h)^{k_3}}{k_1!k_2!k_3!}\]
\pagebreak

\end{document}
